src/SLImp/ImpDependencies.v
@@ -1,7 +1,6 @@
 Require Export SfLib.
 
-Inductive id : Type := 
-  Id : nat -> id.
+Definition id := nat.
 
 Definition state := id -> nat.
 
@@ -10,14 +9,27 @@ Definition empty_state : state :=
   
 Definition beq_id X1 X2 :=
   match (X1, X2) with
-    (Id n1, Id n2) => beq_nat n1 n2
+    (n1, n2) => beq_nat n1 n2
+  end.
+  
+Definition blt_nat (n m : nat) : bool :=
+  match ble_nat n m with
+  | false => false
+  | true => 
+      match beq_nat n m with
+  	    | true => false
+  		| false => true
+  	  end
   end.
 
 Theorem beq_id_refl : forall X,
   true = beq_id X X.
 Proof.
   intros. destruct X.
-  apply beq_nat_refl.  Qed.
+  apply beq_nat_refl. 
+  unfold beq_id.
+  apply beq_nat_refl.
+   Qed.
  
 Definition update (st : state) (X:id) (n : nat) : state :=
   fun X' => if beq_id X X' then n else st X'.
@@ -47,7 +59,11 @@ Proof.
   intros.
   destruct i1. destruct i2.
   apply beq_nat_eq in H.
-  rewrite H. reflexivity.
+  reflexivity.
+  inversion H.
+  unfold beq_id in H.
+  apply beq_nat_eq.
+  assumption.
 Qed.
 
 Theorem update_same : forall x1 k1 k2 (f : state),
